\section{Dynamical System: Analytic Solution}

To study the dynamics of the system, we need to consider the complete diffusion equation, along with the time dependent electric potential equation.

We consider

\begin{align}
\frac{\partial C_+}{\partial t} &= D_+ \left[\nabla^2 C_+ -  \nabla (C_+ \nabla \Psi) \right] , \\
\frac{\partial C_-}{\partial t} &= D_- \left[\nabla^2 C_- + \nabla (C_- \nabla \Psi) \right], \\
\nabla^2 \Psi &= -\kappa^2 \left(C_+ - C_- \right).
\label{eq:dynamic-system}
\end{align}

subject to the border condition 
\begin{align}
C_+(0, x) & = C^{SS}_+(x)\\
C_-(0, x) & =  C^{SS}_-(x)\\\
\Phi(0, x) &= \Phi^{SS}_+(x)\
\end{align}

where the super-script $SS$ indicates the steady state solution (See Ch. 2)%\ref{ch:2).

\subsection{Diffusion Only}

As a first approach to our problem, we evaluate the simpler diffusion-only problem



\begin{align}
\frac{\partial C_+}{\partial t} &= D_+ \nabla^2 C_+,\\
\frac{\partial C_-}{\partial t} &= D_- \nabla^2 C_-,
\label{eq:diffusion}
\end{align}

which in our limit (infinite plate) we can write it as


\begin{align}
\frac{\partial C_s}{\partial t} &= D_+ \frac{\partial^2 C_s}{\partial x^2},\\
\label{eq:diffusion-1d}
\end{align}

with $s=\pm$. The equation is subject to the following boundary conditions


\begin{align}
C(\delta, t) = C_b,\\
J(0,t) = D_s\frac{\partial C}{\partial x}\big|_{x=0} = r\delta_{+,s},
\label{eq:diffusion-bc}
\end{align}

where $J(x,t)$ is the flux.

First, we solve for $s=-$. Let 
\begin{align}
	\rho_-(x,t) &= C_s(x,t) - C_b,\\
	D_-\frac{\partial \rho_-}{\partial x}\big|_{x=0} &= J(0, t) = 0.
\end{align}

Considering the previous change of variables, we know need to solve the system

\begin{align}
\frac{\partial \rho_s}{\partial t} &= D_+ \frac{\partial^2 \rho_s}{\partial x^2},\\
\label{eq:diffusion-1d}
\end{align}


We will solve this equation using the method of separation of variables. Let

\begin{align}
	\rho_-(x,t) = g_-(t)f_-(x)
\end{align}

We get the following two equations for $g_-(t)$ and $f_-(x)$


\begin{align}
	g_-'(t) - \lambda g_-(t) &= 0,\\
	f_-''(x) - \frac{\lambda}{D_-} f_-(t) &= 0.
\end{align}

$\lambda$ is a positive constant. The solution to these equations are

\begin{align}
	g_-(t) =& G_{-,0}e^{\lambda t},\\
	f_-(x) =& F^1_{-,\lambda}\cos\qty{{\sqrt{\frac{\lambda}{D_-}} x}} + F^2_{-,\lambda}\sin\qty{\sqrt{\frac{\lambda}{D_-}} x},
\end{align}

where $F^1_{-,\lambda}$, $F^2_{-,\lambda}$ and $G_{-,0}$ are constants dependent on the parameter $\lambda$, which is yet to be determined. Border conditions \ref{eq:diffusion-1d} yield $B_{-,\lambda} = 0$. We get the general solution,


\begin{align}
	\rho_-(x,t) = \sum_{\lambda} A_\lambda e^{\lambda t} \cos\qty{\frac{\lambda}{D_-} x}
\end{align}

Considering the border condition at $x=\delta$, we can determine the value of $\lambda$,


\begin{align}
	\rho_-(x=\delta,t) = \sum_{\lambda} A_\lambda e^{\lambda t} \cos\qty{\frac{\lambda}{D_-} \delta} = 0.
	\label{bc-delta}
\end{align}

The only way for equation \ref{bc-delta} to be zero is if we get

\begin{align}\nonumber
	\cos\qty{\frac{\lambda}{D_-} \delta} = \frac{(2n+1)\pi}{2}
\end{align}


\begin{align}
	\lambda = \frac{(2n+1)\pi}{2\delta^2}D_-.
\end{align}

The general solution is


\begin{align}
	\rho_-(x,t) = \sum_{n} A_n e^{\frac{(2n+1)\pi}{2\delta^2}D_- t} \cos\qty{\sqrt{\frac{(2n+1)\pi}{2\delta^2}} x}
	\label{bc-delta}
\end{align}

Consider the initial condition as

\begin{align}
	C_-(x,0) = 0 \rightarrow \rho_-(x,0) = -C_b.
\end{align}

Finally, we get

\begin{align}
	\rho_- (x,t) = -C_b\sum_{n}e^{\frac{(2n+1)\pi}{2\delta^2}D_- t} \cos\qty{\sqrt{\frac{(2n+1)\pi}{2\delta^2}} x}.
\end{align}

The concentration is then,

\begin{align}
	C_- (x,t) =C_b\qty{1-\sum_{n}e^{\frac{(2n+1)\pi}{2\delta^2}D_- t} \cos\qty{\sqrt{\frac{(2n+1)\pi}{2\delta^2}} x}}
\end{align}





